Fixed bv_straight.bpl verification under Boogie. The problem was that the attribute was not quite written correctly so the bv8add and bv8ugt function were being treated as uninterpret functions.
The boogie reference manual uses something like
{:bvBuiltin "bvadd8"} which doesn't seem to work. The manual should
be fixed and really a list of smt2 functions to map should be provided.
Are these just SMT-LIB-v2 function names?

test_programs/basic/concrete/bv_straight.bpl
@@ -1,8 +1,8 @@
 procedure main() returns (r:bv8);
 
 // Bitvector functions
-function {:bvBuiltin "bvadd"} bv8add(bv8,bv8) returns(bv8);
-function {:bvBuiltin "bvugt"} bv8ugt(bv8,bv8) returns(bool);
+function {:bvbuiltin "bvadd"} bv8add(bv8,bv8) returns(bv8);
+function {:bvbuiltin "bvugt"} bv8ugt(bv8,bv8) returns(bool);
 
 implementation main() returns (r:bv8)
 {
@@ -11,5 +11,5 @@ implementation main() returns (r:bv8)
     a := 1bv8;
     b := 2bv8;
     r := bv8add(a,b);
-    assert bv8ugt(r, 0bv8); // FIXME: Boogie can't verify
+    assert bv8ugt(r, 0bv8);
 }
